books/projects/atomic-stobjs/lemmas/hash-table$c.lisp
@@ -1,0 +1,731 @@
+;;; Copyright 2025 J. David Taylor
+;;;
+;;; Redistribution and use in source and binary forms, with or without
+;;; modification, are permitted provided that the following conditions are met:
+;;;
+;;; 1. Redistributions of source code must retain the above copyright notice,
+;;;    this list of conditions and the following disclaimer.
+;;;
+;;; 2. Redistributions in binary form must reproduce the above copyright notice,
+;;;    this list of conditions and the following disclaimer in the documentation
+;;;    and/or other materials provided with the distribution.
+;;;
+;;; 3. Neither the name of the copyright holder nor the names of its
+;;;    contributors may be used to endorse or promote products derived from this
+;;;    software without specific prior written permission.
+;;;
+;;; THIS SOFTWARE IS PROVIDED BY THE COPYRIGHT HOLDERS AND CONTRIBUTORS "AS IS"
+;;; AND ANY EXPRESS OR IMPLIED WARRANTIES, INCLUDING, BUT NOT LIMITED TO, THE
+;;; IMPLIED WARRANTIES OF MERCHANTABILITY AND FITNESS FOR A PARTICULAR PURPOSE
+;;; ARE DISCLAIMED. IN NO EVENT SHALL THE COPYRIGHT HOLDER OR CONTRIBUTORS BE
+;;; LIABLE FOR ANY DIRECT, INDIRECT, INCIDENTAL, SPECIAL, EXEMPLARY, OR
+;;; CONSEQUENTIAL DAMAGES (INCLUDING, BUT NOT LIMITED TO, PROCUREMENT OF
+;;; SUBSTITUTE GOODS OR SERVICES; LOSS OF USE, DATA, OR PROFITS; OR BUSINESS
+;;; INTERRUPTION) HOWEVER CAUSED AND ON ANY THEORY OF LIABILITY, WHETHER IN
+;;; CONTRACT, STRICT LIABILITY, OR TORT (INCLUDING NEGLIGENCE OR OTHERWISE)
+;;; ARISING IN ANY WAY OUT OF THE USE OF THIS SOFTWARE, EVEN IF ADVISED OF THE
+;;; POSSIBILITY OF SUCH DAMAGE.
+
+
+(in-package "LEM-HASH-TABLE$C")
+(set-verify-guards-eagerness 2)
+
+#||
+(include-book "std/lists/top" :dir :system)
+(include-book "std/alists/top" :dir :system)
+||#
+
+(include-book "../utilities/with-books")
+(local
+  (include-book "std"))
+
+(encapsulate (((key-guard *) => *)
+              ((element-recognizer *) => *)
+              ((default-value) => *))
+  (local
+    (defun key-guard (key)
+      (declare (xargs :guard t))
+      (symbolp key)))
+
+  (defthm key-guard-constraint
+    (booleanp (key-guard key))
+    :rule-classes :type-prescription)
+
+  (local
+    (defun element-recognizer (value)
+      (declare (xargs :guard t))
+      (symbolp value)))
+
+  (defthm element-recognizer-constraint
+    (booleanp (element-recognizer value))
+    :rule-classes :type-prescription)
+
+  (local
+    (defun default-value ()
+      (declare (xargs :guard t))
+      '||))
+
+  (defthm default-value-constraint
+    (element-recognizer (default-value))))
+
+(defun contents-recognizer (contents)
+  (declare (xargs :guard t))
+  (cond
+    ((atom contents)
+     t)
+    ((consp (car contents))
+     (and (element-recognizer (cdar contents))
+          (contents-recognizer (cdr contents))))
+    (t
+     (contents-recognizer (cdr contents)))))
+
+(defun recognizer (hash-table)
+  (declare (xargs :guard t))
+  (and (true-listp hash-table)
+       (>= (cl::length hash-table) 1)
+       (contents-recognizer (nth 0 hash-table))
+       t))
+
+(defun recognizer/unique (hash-table)
+  (declare (xargs :guard t))
+  (and (true-listp hash-table)
+       (= (cl::length hash-table) 1)
+       (contents-recognizer (nth 0 hash-table))
+       t))
+
+(defun recognizer/copyable (hash-table)
+  (declare (xargs :guard t))
+  (and (true-listp hash-table)
+       (= (cl::length hash-table) 2)
+       (contents-recognizer (nth 0 hash-table))
+       t))
+
+(defun creator/unique ()
+  (declare (xargs :guard t))
+  (list nil))
+
+(defun creator/copyable ()
+  (declare (xargs :guard t))
+  (list nil nil))
+
+(defun accessor (key hash-table)
+  (declare (xargs :guard (and (recognizer hash-table)
+                              (key-guard key))))
+  (let ((pair (hons-assoc-equal key (nth 0 hash-table))))
+    (if pair
+        (cdr pair)
+        (default-value))))
+
+(defun updater (key value hash-table)
+  (declare (xargs :guard (and (recognizer hash-table)
+                              (key-guard key)
+                              (element-recognizer value))))
+  (update-nth 0
+              (cons (cons key value)
+                    (nth 0 hash-table))
+              hash-table))
+
+(defun boundp (key hash-table)
+  (declare (xargs :guard (and (recognizer hash-table)
+                              (key-guard key))))
+  (consp (hons-assoc-equal key (nth 0 hash-table))))
+
+(defun getp (key hash-table)
+  (declare (xargs :guard (and (recognizer hash-table)
+                              (key-guard key))))
+  (mv (accessor key hash-table)
+      (boundp key hash-table)))
+
+(defun remover (key hash-table)
+  (declare (xargs :guard (and (recognizer hash-table)
+                              (key-guard key))))
+  (update-nth 0
+              (hons-remove-assoc key (nth 0 hash-table))
+              hash-table))
+
+(defun count (hash-table)
+  (declare (xargs :guard (recognizer hash-table)))
+  (count-keys (nth 0 hash-table)))
+
+(defun %clear (hash-table)
+  (declare (xargs :guard (recognizer hash-table)))
+  (update-nth 0 nil hash-table))
+
+(defun %init (ht-size rehash-size rehash-threshold hash-table)
+  (declare (xargs :guard (and (recognizer hash-table)
+                              (or (natp ht-size)
+                                  (not ht-size))
+                              (or (and (rationalp rehash-size)
+                                       (<= 1 rehash-size))
+                                  (not rehash-size))
+                              (or (and (rationalp rehash-threshold)
+                                       (<= 0 rehash-threshold)
+                                       (<= rehash-threshold 1))
+                                  (not rehash-threshold))))
+           (ignorable ht-size rehash-size rehash-threshold))
+  (update-nth 0 nil hash-table))
+
+(defun keys (hash-table)
+  (declare (xargs :guard (recognizer/copyable hash-table)))
+  (nth 1 hash-table))
+
+(defun keys-set (set hash-table)
+  (declare (xargs :guard (recognizer/copyable hash-table)))
+  (update-nth 1 set hash-table))
+
+
+;;;; `CONTENTS-RECOGNIZER'
+(defthm contents-recognizer{type-prescription}
+  (booleanp (contents-recognizer contents))
+  :rule-classes :type-prescription)
+
+(local
+  (defthm contents-recognizer-of-hons-remove-assoc
+    (implies (contents-recognizer contents)
+             (contents-recognizer (hons-remove-assoc key contents)))))
+
+(local
+  (defthm element-recognizer-of-cdr-of-hons-assoc-equal
+    (implies (and (contents-recognizer contents)
+                  (hons-assoc-equal key contents))
+             (element-recognizer (cdr (hons-assoc-equal key contents))))))
+
+
+;;;; `RECOGNIZER/UNIQUE'
+(defthm recognizer/unique{type-prescription}
+  (booleanp (recognizer/unique hash-table))
+  :rule-classes :type-prescription)
+
+(defthm recognizer/unique{compound-recognizer}
+  (implies (recognizer/unique hash-table)
+           (and (consp hash-table)
+                (true-listp hash-table)))
+  :rule-classes :compound-recognizer)
+
+(defthm recognizer/unique-of-creator/unique
+  (recognizer/unique (creator/unique)))
+
+(defthm recognizer/unique-of-updater
+  (implies (and (recognizer/unique hash-table)
+                (element-recognizer value))
+           (recognizer/unique (updater key value hash-table))))
+
+(defthm recognizer/unique-of-remover
+  (implies (recognizer/unique hash-table)
+           (recognizer/unique (remover key hash-table))))
+
+(defthm recognizer/unique-of-%clear
+  (implies (recognizer/unique hash-table)
+           (recognizer/unique (%clear hash-table))))
+
+(defthm recognizer/unique-of-%init
+  (implies (recognizer/unique hash-table)
+           (recognizer/unique (%init ht-size rehash-size rehash-threshold hash-table))))
+
+
+;;;; `RECOGNIZER/COPYABLE'
+(defthm recognizer/copyable{type-prescription}
+  (booleanp (recognizer/copyable hash-table))
+  :rule-classes :type-prescription)
+
+(defthm recognizer/copyable{compound-recognizer}
+  (implies (recognizer/copyable hash-table)
+           (and (consp hash-table)
+                (true-listp hash-table)))
+  :rule-classes :compound-recognizer)
+
+(defthm recognizer/copyable-of-creator/copyable
+  (recognizer/copyable (creator/copyable)))
+
+(defthm recognizer/copyable-of-updater
+  (implies (and (recognizer/copyable hash-table)
+                (element-recognizer value))
+           (recognizer/copyable (updater key value hash-table))))
+
+(defthm recognizer/copyable-of-remover
+  (implies (recognizer/copyable hash-table)
+           (recognizer/copyable (remover key hash-table))))
+
+(defthm recognizer/copyable-of-%clear
+  (implies (recognizer/copyable hash-table)
+           (recognizer/copyable (%clear hash-table))))
+
+(defthm recognizer/copyable-of-%init
+  (implies (recognizer/copyable hash-table)
+           (recognizer/copyable (%init ht-size rehash-size rehash-threshold hash-table))))
+
+(defthm recognizer/copyable-of-keys-set
+  (implies (recognizer/copyable hash-table)
+           (recognizer/copyable (keys-set set hash-table))))
+
+
+;;;; `ACCESSOR'
+(defthm element-recognizer-of-accessor/unique
+  (implies (recognizer/unique hash-table)
+           (element-recognizer (accessor key hash-table))))
+
+(defthm element-recognizer-of-accessor/copyable
+  (implies (recognizer/copyable hash-table)
+           (element-recognizer (accessor key hash-table))))
+
+(defthm accessor-of-creator/unique
+  (equal (accessor key (creator/unique))
+         (default-value)))
+
+(defthm accessor-of-creator/copyable
+  (equal (accessor key (creator/copyable))
+         (default-value)))
+
+(defthm accessor-of-updater-same
+  (implies (equal key0 key1)
+           (equal (accessor key0 (updater key1 value hash-table))
+                  value)))
+
+(defthm accessor-of-updater-diff
+  (implies (not (equal key0 key1))
+           (equal (accessor key0 (updater key1 value hash-table))
+                  (accessor key0 hash-table))))
+
+(defthm accessor-of-updater
+  (equal (accessor key0 (updater key1 value hash-table))
+         (if (equal key0 key1)
+             value
+             (accessor key0 hash-table)))
+  :hints
+  (("Goal"
+    :cases ((equal key0 key1)))
+   ("Subgoal 2"
+    :by accessor-of-updater-diff)
+   ("Subgoal 1"
+    :by accessor-of-updater-same)))
+
+(defthm accessor-when-not-boundp
+  (implies (not (boundp key hash-table))
+           (equal (accessor key hash-table)
+                  (default-value))))
+
+(with-books (("std/alists/hons-remove-assoc" :dir :system))
+  (defthm accessor-of-remover-same
+    (implies (equal key0 key1)
+             (equal (accessor key0 (remover key1 hash-table))
+                    (default-value))))
+
+  (defthm accessor-of-remover-diff
+    (implies (not (equal key0 key1))
+             (equal (accessor key0 (remover key1 hash-table))
+                    (accessor key0 hash-table)))))
+
+(defthm accessor-of-remover
+  (equal (accessor key0 (remover key1 hash-table))
+         (if (equal key0 key1)
+             (default-value)
+             (accessor key0 hash-table)))
+  :hints
+  (("Goal"
+    :cases ((equal key0 key1)))
+   ("Subgoal 2"
+    :by accessor-of-remover-diff)
+   ("Subgoal 1"
+    :by accessor-of-remover-same)))
+
+(defthm accessor-of-keys-set
+  (equal (accessor key (keys-set set hash-table))
+         (accessor key hash-table)))
+
+
+;;;; `UPDATER'
+(defthm updater{type-prescription}/unique
+  (implies (recognizer/unique hash-table)
+           (and (consp (updater key value hash-table))
+                (true-listp (updater key value hash-table))))
+  :rule-classes :type-prescription)
+
+(defthm updater{type-prescription}/copyable
+  (implies (recognizer/copyable hash-table)
+           (and (consp (updater key value hash-table))
+                (true-listp (updater key value hash-table))))
+  :rule-classes :type-prescription)
+
+
+;;;; `BOUNDP'
+(defthm boundp{type-prescription}
+  (booleanp (boundp key hash-table))
+  :rule-classes :type-prescription)
+
+(defthm boundp-of-creator/unique
+  (not (boundp key (creator/unique))))
+
+(defthm boundp-of-creator/copyable
+  (not (boundp key (creator/copyable))))
+
+(defthm boundp-of-updater-same
+  (implies (equal key0 key1)
+           (equal (boundp key0 (updater key1 value hash-table))
+                  t)))
+
+(defthm boundp-of-updater-diff
+  (implies (not (equal key0 key1))
+           (equal (boundp key0 (updater key1 value hash-table))
+                  (boundp key0 hash-table))))
+
+(defthm boundp-of-updater
+  (equal (boundp key0 (updater key1 value hash-table))
+         (or (equal key0 key1)
+             (boundp key0 hash-table)))
+  :hints
+  (("Goal"
+    :cases ((equal key0 key1)))
+   ("Subgoal 2"
+    :by boundp-of-updater-diff)
+   ("Subgoal 1"
+    :use boundp-of-updater-same)))
+
+(with-books (("std/alists/hons-remove-assoc" :dir :system))
+  (defthm boundp-of-remover-same
+    (implies (equal key0 key1)
+             (not (boundp key0 (remover key1 hash-table)))))
+
+  (defthm boundp-of-remover-diff
+    (implies (not (equal key0 key1))
+             (equal (boundp key0 (remover key1 hash-table))
+                    (boundp key0 hash-table)))))
+
+(defthm boundp-of-remover
+  (equal (boundp key0 (remover key1 hash-table))
+         (if (equal key0 key1)
+             nil
+             (boundp key0 hash-table)))
+  :hints
+  (("Goal"
+    :cases ((equal key0 key1)))
+   ("Subgoal 2"
+    :by boundp-of-remover-diff)
+   ("Subgoal 1"
+    :use boundp-of-remover-same)))
+
+(defthm boundp-of-keys-set
+  (equal (boundp key (keys-set set hash-table))
+         (boundp key hash-table)))
+
+
+;;;; `GETP'
+(defthm getp{type-prescription}
+  (and (consp (getp key hash-table))
+       (true-listp (getp key hash-table)))
+  :rule-classes :type-prescription)
+
+(defthm getp{rewrite}
+  (mv-let (v0 v1)
+          (getp key hash-table)
+    (and (equal v0 (accessor key hash-table))
+         (equal v1 (boundp key hash-table)))))
+
+
+;;;; `REMOVER'
+(defthm remover{type-prescription}/unique
+  (implies (recognizer/unique hash-table)
+           (and (consp (remover key hash-table))
+                (true-listp (remover key hash-table))))
+  :rule-classes :type-prescription)
+
+(defthm remover{type-prescription}/copyable
+  (implies (recognizer/copyable hash-table)
+           (and (consp (remover key hash-table))
+                (true-listp (remover key hash-table))))
+  :rule-classes :type-prescription)
+
+(defthm remover-of-creator/unique
+  (equal (remover key (creator/unique))
+         (creator/unique)))
+
+(defthm remover-of-creator/copyable
+  (equal (remover key (creator/copyable))
+         (creator/copyable)))
+
+(defthm remover-of-updater-same
+  (implies (equal key0 key1)
+           (equal (remover key0 (updater key1 value hash-table))
+                  (remover key0 hash-table))))
+
+(defthm remover-of-updater-diff
+  (implies (not (equal key0 key1))
+           (equal (remover key0 (updater key1 value hash-table))
+                  (updater key1 value (remover key0 hash-table)))))
+
+(defthm remover-of-updater
+  (equal (remover key0 (updater key1 value hash-table))
+         (if (equal key0 key1)
+             (remover key0 hash-table)
+             (updater key1 value (remover key0 hash-table))))
+  :hints
+  (("Goal"
+    :cases ((equal key0 key1)))
+   ("Subgoal 2"
+    :by remover-of-updater-diff)
+   ("Subgoal 1"
+    :by remover-of-updater-same)))
+
+(with-books (("std/alists/hons-remove-assoc" :dir :system))
+  (defthm remover-of-remover-same
+    (implies (equal key0 key1)
+             (equal (remover key0 (remover key1 hash-table))
+                    (remover key0 hash-table))))
+
+  (defthm remover-of-remover-diff
+    (implies (not (equal key0 key1))
+             (equal (remover key0 (remover key1 hash-table))
+                    (remover key1 (remover key0 hash-table))))
+    :rule-classes
+    ((:rewrite :loop-stopper ((key0 key1 remover))))))
+
+
+;;;; `COUNT'
+(defthm count{type-prescription}
+  (natp (count hash-table))
+  :rule-classes :type-prescription)
+
+(defthm count-of-creator/unique
+  (equal (count (creator/unique)) 0))
+
+(defthm count-of-creator/copyable
+  (equal (count (creator/copyable)) 0))
+
+(defthm count-of-updater-when-boundp
+  (implies (boundp key hash-table)
+           (equal (count (updater key value hash-table))
+                  (count hash-table))))
+
+(defthm count-of-updater-when-not-boundp
+  (implies (not (boundp key hash-table))
+           (equal (count (updater key value hash-table))
+                  (1+ (count hash-table)))))
+
+(defthm count-of-updater
+  (equal (count (updater key value hash-table))
+         (if (boundp key hash-table)
+             (count hash-table)
+             (1+ (count hash-table))))
+  :hints
+  (("Goal"
+    :cases ((boundp key hash-table)))
+   ("Subgoal 2"
+    :by count-of-updater-when-not-boundp)
+   ("Subgoal 1"
+    :by count-of-updater-when-boundp)))
+
+(defthm count-when-boundp
+  (implies (boundp key hash-table)
+           (posp (count hash-table)))
+  :rule-classes :type-prescription)
+
+(defthm count-of-remover-when-boundp
+  (implies (boundp key hash-table)
+           (equal (count (remover key hash-table))
+                  (1- (count hash-table)))))
+
+(defthm count-of-remover-when-not-boundp
+  (implies (not (boundp key hash-table))
+           (equal (count (remover key hash-table))
+                  (count hash-table))))
+
+(defthm count-of-remover
+  (equal (count (remover key hash-table))
+         (if (boundp key hash-table)
+             (1- (count hash-table))
+             (count hash-table)))
+  :hints
+  (("Goal"
+    :cases ((boundp key hash-table)))
+   ("Subgoal 2"
+    :by count-of-remover-when-not-boundp)
+   ("Subgoal 1"
+    :by count-of-remover-when-boundp)))
+
+(defthm count-of-keys-set
+  (equal (count (keys-set set hash-table))
+         (count hash-table)))
+
+
+;;;; `%CLEAR'
+(defthm %clear{type-prescription}/unique
+  (implies (recognizer/unique hash-table)
+           (and (consp (%clear hash-table))
+                (true-listp (%clear hash-table))))
+  :rule-classes :type-prescription)
+
+(defthm %clear{type-prescription}/copyable
+  (implies (recognizer/copyable hash-table)
+           (and (consp (%clear hash-table))
+                (true-listp (%clear hash-table))))
+  :rule-classes :type-prescription)
+
+(with-books (("std/lists/len" :dir :system)
+             ("std/lists/nth" :dir :system))
+  (defthm %clear{rewrite}/unique
+    (implies (recognizer/unique hash-table)
+             (equal (%clear hash-table)
+                    (creator/unique))))
+
+  (defthm %clear{rewrite}/copyable
+    (implies (recognizer/copyable hash-table)
+             (equal (%clear hash-table)
+                    (keys-set (keys hash-table) (creator/copyable))))
+    :hints
+    ((acl2::equal-by-nths-hint))))
+
+
+;;;; `%INIT'
+(defthm %init{type-prescription}/unique
+  (implies (recognizer/unique hash-table)
+           (and (consp (%init ht-size rehash-size rehash-threshold hash-table))
+                (true-listp (%init ht-size rehash-size rehash-threshold hash-table))))
+  :rule-classes :type-prescription)
+
+(defthm %init{type-prescription}/copyable
+  (implies (recognizer/copyable hash-table)
+           (and (consp (%init ht-size rehash-size rehash-threshold hash-table))
+                (true-listp (%init ht-size rehash-size rehash-threshold hash-table))))
+  :rule-classes :type-prescription)
+
+(with-books (("std/lists/len" :dir :system)
+             ("std/lists/nth" :dir :system))
+  (defthm %init{rewrite}/unique
+    (implies (recognizer/unique hash-table)
+             (equal (%init ht-size rehash-size rehash-threshold hash-table)
+                    (creator/unique))))
+
+  (defthm %init{rewrite}/copyable
+    (implies (recognizer/copyable hash-table)
+             (equal (%init ht-size rehash-size rehash-threshold hash-table)
+                    (keys-set (keys hash-table) (creator/copyable))))
+    :hints
+    ((acl2::equal-by-nths-hint))))
+
+
+;;;; `KEYS'
+(defthm keys-of-creator/unique
+  (not (keys (creator/unique))))
+
+(defthm keys-of-creator/copyable
+  (not (keys (creator/copyable))))
+
+(defthm keys-of-updater
+  (equal (keys (updater key value hash-table))
+         (keys hash-table)))
+
+(defthm keys-of-remover
+  (equal (keys (remover key hash-table))
+         (keys hash-table)))
+
+(defthm keys-of-keys-set
+  (equal (keys (keys-set set hash-table))
+         set))
+
+
+;;;; `KEYS-SET'
+(defthm keys-set{type-prescription}
+  (implies (recognizer/copyable hash-table)
+           (and (consp (keys-set set hash-table))
+                (true-listp (keys-set set hash-table))))
+  :rule-classes :type-prescription)
+
+(with-books (("std/lists/update-nth" :dir :system))
+  (defthm keys-set-of-updater
+    (equal (keys-set set (updater key value hash-table))
+           (updater key value (keys-set set hash-table))))
+
+  (defthm keys-set-of-remover
+    (equal (keys-set set (remover key hash-table))
+           (remover key (keys-set set hash-table))))
+
+  (defthm keys-set-of-keys-set
+    (equal (keys-set %set (keys-set set hash-table))
+           (keys-set %set hash-table))))
+
+
+;;;; `FIXER/UNIQUE'
+(defun fixer/unique (hash-table)
+  (declare (xargs :guard (recognizer/unique hash-table)))
+  (if (recognizer/unique hash-table)
+      hash-table
+      (creator/unique)))
+
+(defthm fixer/unique{type-prescription}
+  (and (consp (fixer/unique hash-table))
+       (true-listp (fixer/unique hash-table)))
+  :rule-classes :type-prescription)
+
+(defthm recognizer/unique-of-fixer/unique
+  (recognizer/unique (fixer/unique hash-table)))
+
+(defthm fixer/unique-when-recognizer/unique
+  (implies (recognizer/unique hash-table)
+           (equal (fixer/unique hash-table)
+                  hash-table)))
+
+(defthm fixer/unique-when-not-recognizer/unique
+  (implies (not (recognizer/unique hash-table))
+           (equal (fixer/unique hash-table)
+                  (creator/unique))))
+
+
+;;;; `FIXER/COPYABLE'
+(defun fixer/copyable (hash-table)
+  (declare (xargs :guard (recognizer/copyable hash-table)))
+  (if (recognizer/copyable hash-table)
+      hash-table
+      (creator/copyable)))
+
+(defthm fixer/copyable{type-prescription}
+  (and (consp (fixer/copyable hash-table))
+       (true-listp (fixer/copyable hash-table)))
+  :rule-classes :type-prescription)
+
+(defthm recognizer/copyable-of-fixer/copyable
+  (recognizer/copyable (fixer/copyable hash-table)))
+
+(defthm fixer/copyable-when-recognizer/copyable
+  (implies (recognizer/copyable hash-table)
+           (equal (fixer/copyable hash-table)
+                  hash-table)))
+
+(defthm fixer/copyable-when-not-recognizer/copyable
+  (implies (not (recognizer/copyable hash-table))
+           (equal (fixer/copyable hash-table)
+                  (creator/copyable))))
+
+
+;;;; `CLEAR'
+(defun clear (hash-table)
+  (declare (xargs :guard (recognizer/copyable hash-table)))
+  (%clear (keys-set '() (fixer/copyable hash-table))))
+
+(with-books (("std/lists/len" :dir :system)
+             ("std/lists/update-nth" :dir :system))
+  (defthm clear{rewrite}
+    (implies (recognizer/copyable hash-table)
+             (equal (clear hash-table)
+                    (creator/copyable)))))
+
+
+;;;; `INIT'
+(defun init (ht-size rehash-size rehash-threshold hash-table)
+  (declare (xargs :guard (and (recognizer/copyable hash-table)
+                              (or (natp ht-size)
+                                  (not ht-size))
+                              (or (and (rationalp rehash-size)
+                                       (<= 1 rehash-size))
+                                  (not rehash-size))
+                              (or (and (rationalp rehash-threshold)
+                                       (<= 0 rehash-threshold)
+                                       (<= rehash-threshold 1))
+                                  (not rehash-threshold)))))
+  (%init ht-size rehash-size rehash-threshold
+         (keys-set '() (fixer/copyable hash-table))))
+
+(with-books (("std/lists/len" :dir :system)
+             ("std/lists/update-nth" :dir :system))
+  (defthm init{rewrite}
+    (implies (recognizer/copyable hash-table)
+             (equal (init ht-size rehash-size rehash-threshold hash-table)
+                    (creator/copyable)))))
